{
 "cells": [
  {
   "cell_type": "markdown",
   "id": "0e199ea4-1917-45b2-a155-a3824545871f",
   "metadata": {},
   "source": [
    "### PRML 1.2 Probability Theory\n",
    "\n",
    "**Joint probability of X and Y:**\n",
    "\n",
    "$p(X = x_{\\text{$i$}}, Y = y_{\\text{$j$}}) = \\frac{n_{\\text{$ij$}}}{N}$\n",
    "\n",
    "Here, $n_{\\text{$ij$}}$ denotes the number of instances where $X = x_{\\text{$i$}}$ and $Y = y_{\\text{$j$}}$. Dividing this by the total N trials gives the probability that both $x_{\\text{$i$}}$ and $y_{\\text{$j$}}$ happen at the same instance.\n",
    "\n",
    "Visualize a grid with $j$-th rows and $i$-th columns, then $n_{\\text{$ij$}}$ is a cell inside this grid, $c_{\\text{$i$}}$ is a column and $r_{\\text{$j$}}$ is a row. $c$ and $r$ denote the number of  trials where $X = x_{\\text{$i$}}$ and $Y = y_{\\text{$j$}}$ hold respectively.\n",
    "\n",
    " \n",
    "**Sum Rule**\n",
    "\n",
    "$p(X = x_{\\text{$i$}}) = \\frac{c_{i}}{N}$ takes any value in the column $c_{i}$, regardless of the row. This means $c_{\\text{$i$}}$ is equal to the sum of every cell $n_{ij}$ in the column: $c_{\\text{$i$}} = \\sum\\limits_{j} n_{ij}$\n",
    "\n",
    "Substituting this into $p(X = x_{i})$ gives: \n",
    "\n",
    "$p(X = x_{i}) = \\frac{\\sum\\limits_{j} n_{ij}}{N}$\n",
    "\n",
    "Since $N$ is a constant, this formula can be rewritten as the **sum rule**:\n",
    "\n",
    "$p(X = x_{i}) = \\sum\\limits_{j=1}^{L} p(X = x_{\\text{$i$}}, Y = y_{\\text{$j$}})$\n",
    "\n",
    "**Conditional Probability**\n",
    "Given the instances for which $X = x_{i}$, every instance where $Y = y_{j}$ holds as well, is called the conditional probability of Y, given X:\n",
    "\n",
    "$p(Y = y_{j} | X = x_{i}) = \\frac{n_{ij}}{c_{i}}$\n",
    "\n",
    "**Product Rule**\n",
    "The product rule can be derived from the following relationship:\n",
    "\n",
    "$$\n",
    "p(X = x_{i}, Y = y_{j}) = \\frac{n_{ij}}{N} = \\frac{c_{i} \\cdot n_{ij}}{c_{i} \\cdot N} = \\frac{n_{ij}}{c_{i}} \\cdot \\frac{c_{i}}{N} = p(Y = y_{j} | X = x_{i}) \\cdot p(X = x_{i})\n",
    "$$\n",
    "\n",
    "**Bayes Theorem**\n",
    "The relationship between conditional probabilities can be derived from the product rule:\n",
    "\n",
    "\n",
    "$$\n",
    "p(Y = y_{j} | X = x_{i}) \\cdot p(X = x_{i}) = p(X = x_{i}, Y = y_{j})\n",
    "$$\n",
    "\n",
    "dividing by $p(X = x_{i})$:\n",
    "\n",
    "$$\n",
    "p(Y = y_{j} | X = x_{i}) = \\frac{p(X = x_{i}, Y = y_{j})}{p(X = x_{i})}\n",
    "$$\n",
    "\n",
    "Symmetry property property $p(X,Y) = p(Y,X)$: \n",
    "\n",
    "$$\n",
    "p(Y = y_{j} | X = x_{i}) = \\frac{p(Y = y_{j}, X = x_{i})}{p(X = x_{i})}\n",
    "$$\n",
    "\n",
    "Filling in product rule:\n",
    "\n",
    "$$\n",
    "p(Y = y_{j} | X = x_{i}) = \\frac{p(X = x_{i} | Y = y_{j}) \\cdot p(Y = y_{j})}{p(X = x_{i})}\n",
    "$$\n",
    "\n",
    "Exercise 1.3 \n",
    "\n"
   ]
  },
  {
   "cell_type": "code",
   "execution_count": null,
   "id": "3a4a0103-ed7f-4340-b90a-2ae467d6ac1c",
   "metadata": {},
   "outputs": [],
   "source": []
  },
  {
   "cell_type": "code",
   "execution_count": null,
   "id": "020fba62-fb39-47e9-90cb-4cc0590ee037",
   "metadata": {},
   "outputs": [],
   "source": []
  }
 ],
 "metadata": {
  "kernelspec": {
   "display_name": "Python 3 (ipykernel)",
   "language": "python",
   "name": "python3"
  },
  "language_info": {
   "codemirror_mode": {
    "name": "ipython",
    "version": 3
   },
   "file_extension": ".py",
   "mimetype": "text/x-python",
   "name": "python",
   "nbconvert_exporter": "python",
   "pygments_lexer": "ipython3",
   "version": "3.11.7"
  }
 },
 "nbformat": 4,
 "nbformat_minor": 5
}
